intermediate commit

SimulationDiv.thy
@@ -10,52 +10,58 @@ text {*
   We formalize a notion of simulation with divergences on LTSes. This formalization is carried
   out having in mind its application to the concept of refinement in the B method. In B, when
   a module $R$ refines a module $A$, a simulation-like relation is established from $R$ to $A$,
-  i.e. every action taken by $R$, in response to an event that is considered acceptable by $A$
-  shall be simulated by a corresponding action in $A$.
+  i.e. every action taken by $R$, \emph{in response to an event that is considered acceptable
+  by $A$}, shall be simulated by a corresponding action in $A$.
 
-  It is called a gluing invariant and must be such that $R$ cannot diverge in situations where
-  $A$ does not diverge. But $R$ may well be more "robust" and not diverge in a state where $A$
-  would diverge. Of course, in that cases, the behavior of $R$ is not constrained. In the case
-  where $A$ does not diverge, then $R$ must exhibit a behavior that corresponds to one of the
-  possible behaviors of $A$.
+  Essentially, we want to formalize this as follows: assuming $R$ is a refinement of $A$.
+  For every trace $t_R$ of $R$, there is a trace $t_A$ in $A$, with corresponding divergence
+  set $E_A$, such that $t_A = t_R$ or $t_A \conc e$, with $e in E_A$ is a prefix of $t_R$.  
+
+  Conversely, for every trace $t_A$ of $A$ leading to a state with divergence set $E_A$, 
+  there is a corresponding trace $t_R$ in $R$ (i.e. $t_R = t_A$) with
+  a divergence set $E_R \supseteq E_A$.
+
+  This relation is called a \emph{gluing invariant} and must be such that $R$ shall not diverge 
+  in situations where $A$ does not diverge. But $R$ may well be more "robust" and not diverge in
+  a state where $A$ would diverge. Of course, in that cases, the behavior of $R$ is not 
+  constrained. In the case where $A$ does not diverge, then $R$ must exhibit a behavior that 
+  corresponds to one of the possible behaviors of $A$, i.e. the transition taken on the event
+  leads $R$ to a state where it may still be simulated by $A$.
 
   A simulation with divergence is a relation @{text "r"} between the states of one LTS
   and the states of another LTS such that any transition taken by the former, 
   \emph{on an event that does not cause the latter to diverge}, can be simulated
   by the latter. 
 
-  We say that an event @{text "e"} is \emph{accepted} in a state @{text "s"} of a LTS if @{text "(s, e)"}
-  does not belong to the divergences of the LTS (not formalized).
-
 *}
 
 text {*
+  Notice that the classic notion of transition simulation is symmetric, since it does 
+  not consider possible divergences. This property is no longer desirable when divergences
+  are accounted for. 
   The following function @{text "sim_transition"} lifts a relation on states to
   a relation on transitions: it requires the source and destination states to be
-  related, and the labels to coincide.
+  related, and the labels to coincide. It takes an additional input parameter that
+  corresponds to the set of diverging events. 
 *}
 
+(* original definition *)
 definition sim_transition :: "'st rel \<Rightarrow> ('st, 'ev) Tr rel" where
-  "sim_transition r \<equiv> { (t,t') | t t'. (src t, src t') \<in> r
-                                     \<and> lbl t = lbl t' \<and> (dst t, dst t') \<in> r }"
-
-text {*
-  Notice that this classic notion of transition is symmetric, since it does not consider
-  possible divergences. Next function is an attempt to rephrase the simulation between 
-  transitions taking into account a set of divergences. 
-*}
-
-definition sim_div_transition :: "'st rel \<Rightarrow> ('st * 'ev) set \<Rightarrow> ('st, 'ev) Tr rel" where
-  "sim_div_transition r d \<equiv> 
+  "sim_transition r \<equiv> 
     { (tc,ta) | tc ta. 
-      (src tc, src ta) \<in> r \<and> lbl tc = lbl ta \<and>
-      ((src ta, lbl ta) \<in> d \<or> 
-       (src ta, lbl ta) \<notin> d \<and> (dst tc, dst ta) \<in> r) }"
+      (src tc, src ta) \<in> r \<and> lbl tc = lbl ta \<and> (dst tc, dst ta) \<in> r }"
+
+definition div_sim_transition :: "'st rel \<Rightarrow> ('st * 'ev) set \<Rightarrow> ('st, 'ev) Tr rel" where
+  "div_sim_transition r d \<equiv> 
+    { (tc,ta) | tc ta. 
+      (src tc, src ta) \<in> r \<and> 
+      lbl tc = lbl ta \<and>
+      ((src ta, lbl ta) \<notin> d \<longrightarrow> (tc, ta) \<in> sim_transition r) }"
 
 text {*
   With this definition, if @{text "(sa, e)"} diverges, then any transition from a state 
   @{text "sc"} related to @{text "sa"} by @{text "r"}, and labeled @{text "e"} is 
-  considered simulated.
+  considered to be in the relation.
 *}
 
 text {* 
@@ -72,36 +78,39 @@ text {*
   \end{itemize}
 *}
 
-definition simulation :: "'st rel \<Rightarrow> ('st, 'ev) LTSDiv rel" where
-  "simulation r \<equiv> { (l,l') | l l'.
-     (\<forall>s \<in> init l. \<exists>s' \<in> init l'. (s, s') \<in> r)
-   \<and> (\<forall>s s'. (s, s') \<in> r \<longrightarrow>
-        (\<forall>e . 
-          e \<in> div_state l' s' \<or>
-         (e \<notin> div_state l s \<and> 
-              (\<forall>t \<in> trans l. src t = s \<longrightarrow> lbl t = e \<longrightarrow>
-                   (\<exists>t' \<in> trans l'. src t' = s' \<and> lbl t' = e \<and> (t,t') \<in> sim_transition r))))) }"
-
 text {*
   The definition of simulation with divergences between LTSes can also be phrased using the
-  simulation with divergences on transitions:
+  simulation with divergences on transitions. This new version uses the second definition of
+  transition simulation, and reads more gracefully than the previous version:
 *}
 
-definition simulation_div :: "'st rel \<Rightarrow> ('st, 'ev) LTSDiv rel" where
-  "simulation_div r \<equiv> { (l,l') | l l'.
+definition div_simulation :: "'st rel \<Rightarrow> ('st, 'ev) LTSDiv rel" where
+  "div_simulation r \<equiv> { (l,l') | l l'.
      (\<forall>s \<in> init l. \<exists>s' \<in> init l'. (s, s') \<in> r)
    \<and> (\<forall>s s'. (s, s') \<in> r \<longrightarrow>
         (\<forall>t \<in> trans l. src t = s \<longrightarrow>
            (\<exists>t' \<in> trans l'. src t' = s' \<and> lbl t' = lbl t \<and> 
-              (t,t') \<in> sim_div_transition r (divergences l')))) }"
+              (t,t') \<in> div_sim_transition r (divergences l')))) }"
+
+(* alternative definition: *)
+definition simulation :: "'st rel \<Rightarrow> ('st, 'ev) LTSDiv rel" where
+  "simulation r \<equiv> { (l,l') | l l'.
+     (\<forall>s \<in> init l. \<exists>s' \<in> init l'. (s, s') \<in> r)
+   \<and> (\<forall>s s'. (s, s') \<in> r \<longrightarrow>
+        (\<forall>t \<in> trans l. src t = s \<longrightarrow> (s', lbl t) \<notin> divergences l' \<longrightarrow>
+           (\<exists>t' \<in> trans l'. src t' = s' \<and> lbl t' = lbl t \<and> 
+              (t,t') \<in> sim_transition r))) }"
 
 text {* 
   We say that @{text "l'"} simulates @{text "l"} (through @{text "r"}), or that 
   @{text "l"} is simulated by @{text "l'"} through @{text "r"}, if there is a 
   simulation @{text "r"} from @{text "l"} to @{text "l'"}.
 *}
-definition simulated_by (infixl "\<preceq>" 50)
-where "(l \<preceq> l') \<equiv> \<exists>r. (l,l') \<in> simulation_div r"
+definition div_simulated_by (infixl "\<preceq>" 50)
+where "(l \<preceq> l') \<equiv> \<exists>r. (l,l') \<in> div_simulation r"
+
+definition simulated_by (infixl "\<preceq>\<preceq>" 50)
+where "(l \<preceq>\<preceq> l') \<equiv> \<exists>r. (l,l') \<in> simulation r"
 
 (* A lemma that we might want to prove is the containment of the set of diverging events:
 
@@ -111,6 +120,22 @@ s' \<in> states l' \<longrightarrow>
 (s, s') \<in> r \<longrightarrow>
 div_state l s \<subseteq> div_state l' s'
 *)
+
+(* A lemma that we might want to prove is the containment of the set of diverging events:
+
+l \<preceq> l' \<longrightarrow>
+s \<in> states l \<longrightarrow>
+s' \<in> states l' \<longrightarrow>
+(s, s') \<in> r \<longrightarrow>
+div_state l s \<subseteq> div_state l' s'
+*)
+lemma div_simulation_contains:
+  assumes 
+    "(l, l') \<in> div_simulation r"
+  shows 
+    "div_trans l \<subseteq> div_trans l'"
+using assms unfolding simulation_def div_trans_def sim_transition_def
+sorry (*sledgehammer[verbose, max_facts=100, provers="cvc4 e z3 spass remote_vampire"] *)
 
 subsection {* Properties *}
 
@@ -123,39 +148,47 @@ text {*
 lemma simulation_identity : "(Id::('st,'ev) LTSDiv rel) \<subseteq> simulation (Id::'st rel)" 
   unfolding simulation_def sim_transition_def by auto
 
-lemma simulation_div_identity : "(Id::('st,'ev) LTSDiv rel) \<subseteq> simulation_div (Id::'st rel)" 
-  unfolding simulation_div_def sim_div_transition_def by auto
+lemma div_simulation_identity : "(Id::('st,'ev) LTSDiv rel) \<subseteq> div_simulation (Id::'st rel)" 
+  unfolding div_simulation_def div_sim_transition_def sim_transition_def by auto
 
 text {*
    Second, we have that the composition of two simulation relations is a simulation relation.
 *}
-
 lemma simulation_composition:
   assumes "(l, l') \<in> simulation r" and "(l', l'') \<in> simulation r'"
   shows "(l, l'') \<in> simulation (r O r')"
-using assms unfolding simulation_def
+  using assms unfolding simulation_def
   using assms unfolding sim_transition_def relcomp_unfold
-  by auto (metis+)
+sorry
+(* was: by auto(metis+) *)
 
-lemma simulation_div_composition:
-  assumes "(l, l') \<in> simulation_div r" and "(l', l'') \<in> simulation_div r'"
-  shows "(l, l'') \<in> simulation_div (r O r')"
-using assms unfolding simulation_div_def
-  using assms unfolding sim_div_transition_def relcomp_unfold
-  by auto (metis+)
+lemma div_simulation_composition:
+  assumes "(l, l') \<in> div_simulation r" and "(l', l'') \<in> div_simulation r'"
+  shows "(l, l'') \<in> div_simulation (r O r')"
+  using assms unfolding div_simulation_def
+  using assms unfolding div_sim_transition_def sim_transition_def relcomp_unfold
+sorry
+
 
 text {* 
   These properties are lifted to the simulates relation over LTS.
 *}
 
-lemma simulated_div_by_reflexive: "l \<preceq> l" 
-  unfolding simulated_by_def using simulation_div_identity by blast
+lemma div_simulated_by_reflexive: "l \<preceq> l" 
+  unfolding div_simulated_by_def using div_simulation_identity by blast
 
-lemma simulates_transitive:
+lemma div_simulated_by_transitive:
   assumes "l \<preceq> l'" and "l' \<preceq> l''"
   shows "l \<preceq> l''"
-  using assms unfolding simulated_by_def using simulation_div_composition by blast
+  using assms unfolding div_simulated_by_def using div_simulation_composition by blast
 
+lemma simulated_by_reflexive: "l \<preceq>\<preceq> l" 
+  unfolding simulated_by_def using simulation_identity by (auto)
+
+lemma simulated_by_transitive:
+  assumes "l \<preceq>\<preceq> l'" and "l' \<preceq>\<preceq> l''"
+  shows "l \<preceq>\<preceq> l''"
+  using assms unfolding simulated_by_def using simulation_composition by blast
 
 subsection {* Simulation and behavior *}
 
@@ -163,10 +196,18 @@ text {*
   Similarly, a relation @{text r} on states induces a simulation between two runs:
   corresponding transitions must be related according to @{text r}, lifted to
   transitions.
+
+  If ts is simulated by ts' through r, we only care as long as ts takes transition
+  that do not provoke a divergence in ts.
 *}
+
 definition sim_run :: "'st rel \<Rightarrow> ('st, 'ev) Run rel" where
   "sim_run r \<equiv> {(ts, ts') | ts ts'. 
-                            list_all2 (\<lambda>t t'. (t,t') \<in> sim_transition r) ts ts'}"
+                   list_all2 (\<lambda>t t'. (t,t') \<in> sim_transition r) ts ts'}"
+
+definition div_sim_run :: "'st rel \<Rightarrow> ('st * 'ev) set \<Rightarrow> ('st, 'ev) Run rel" where
+  "div_sim_run r d \<equiv> {(ts, ts') | ts ts'. 
+                            list_all2 (\<lambda>t t'. (t,t') \<in> div_sim_transition r d) ts ts'}"
 
 (* original definition -- note that the one above is weaker because it does
    not enforce that the arguments are actually runs; however, it seems more
@@ -183,57 +224,62 @@ text {*
   If two runs are similar, they have the same length.
   In particular, one is empty iff the other one is.
 *}
-lemma sim_run_eq_length: "(ts, ts') \<in> sim_run r \<Longrightarrow> length ts = length ts'"
-  unfolding sim_run_def by (auto dest: list_all2_lengthD)
 
-lemma sim_run_empty_iff: "(ts, ts') \<in> sim_run r \<Longrightarrow> (ts = [] \<longleftrightarrow> ts' = [])"
-  by (auto dest: sim_run_eq_length)
+lemma div_sim_run_eq_length: "(ts, ts') \<in> div_sim_run r d \<Longrightarrow> length ts = length ts'"
+  unfolding div_sim_run_def by (auto dest: list_all2_lengthD)
 
-lemma sim_run_empty [simp]:
-  "([], ts) \<in> sim_run r = (ts = [])" 
-  "(ts, []) \<in> sim_run r = (ts = [])"
-  unfolding sim_run_def by auto
+lemma div_sim_run_empty_iff: "(ts, ts') \<in> div_sim_run r d \<Longrightarrow> (ts = [] \<longleftrightarrow> ts' = [])"
+  by (auto dest: div_sim_run_eq_length)
+
+lemma div_sim_run_empty [simp]:
+  "([], ts) \<in> div_sim_run r d = (ts = [])" 
+  "(ts, []) \<in> div_sim_run r d = (ts = [])"
+  unfolding div_sim_run_def by auto
 
 text {*
   Two singleton runs are similar if the transitions are related.
 *}
-lemma sim_run_singleton [simp]:
-  "([t], ts) \<in> sim_run r = (\<exists>t'. ts = [t'] \<and> (t,t') \<in> sim_transition r)"
-  "(ts, [t]) \<in> sim_run r = (\<exists>t'. ts = [t'] \<and> (t',t) \<in> sim_transition r)"
-  unfolding sim_run_def by (auto simp: list_all2_Cons1 list_all2_Cons2)
+
+lemma div_sim_run_singleton [simp]:
+  "([t], ts) \<in> div_sim_run r d = (\<exists> t'. ts = [t'] \<and> (t, t') \<in> div_sim_transition r d)"
+  "(ts, [t]) \<in> div_sim_run r d = (\<exists> t'. ts = [t'] \<and> (t', t) \<in> div_sim_transition r d)"
+  unfolding div_sim_run_def by (auto simp:list_all2_Cons1 list_all2_Cons2)
 
 text {*
   For two similar runs, all transitions at corresponding positions are related.
   In particular, the last transitions of two similar, non-empty runs are related,
   as are the last states.
 *}
-lemma sim_run_nth:
-  "(ts, ts') \<in> sim_run r \<Longrightarrow> \<forall>i < length ts. (ts!i, ts'!i) \<in> sim_transition r"
-  by (simp add: sim_run_def list_all2_conv_all_nth)
  
-lemma sim_run_last_trans: 
-  "\<lbrakk> (ts, ts') \<in> sim_run r; ts \<noteq> [] \<rbrakk> \<Longrightarrow> (last ts, last ts') \<in> sim_transition r"
-  by (simp add: last_conv_nth sim_run_empty_iff sim_run_eq_length sim_run_nth)
+lemma div_sim_run_nth:
+  "(ts, ts') \<in> div_sim_run r d \<Longrightarrow> \<forall>i < length ts. (ts!i, ts'!i) \<in> div_sim_transition r d"
+  by (simp add: div_sim_run_def list_all2_conv_all_nth)
 
-lemma sim_run_last_state: 
-  "\<lbrakk> (ts, ts') \<in> sim_run r; ts \<noteq> [] \<rbrakk> \<Longrightarrow> (dst (last ts), dst(last ts')) \<in> r"
-  by (auto dest: sim_run_last_trans simp: sim_transition_def)
+lemma div_sim_run_last_trans: 
+  "\<lbrakk> (ts, ts') \<in> div_sim_run r d; ts \<noteq> [] \<rbrakk> \<Longrightarrow> (last ts, last ts') \<in> div_sim_transition r d"
+  by (simp add: last_conv_nth div_sim_run_empty_iff div_sim_run_eq_length div_sim_run_nth)
+
+lemma div_sim_run_last_state: 
+  "\<lbrakk> (ts, ts') \<in> div_sim_run r d; ts \<noteq> [] \<rbrakk> \<Longrightarrow> 
+     (src (last ts'), lbl(last ts)) \<in> d \<or> ((dst (last ts), dst(last ts')) \<in> r)"
+  by (auto dest: div_sim_run_last_trans simp: div_sim_transition_def simp: sim_transition_def)
 
 text {*
   The concatenation of two similar runs is similar.
 *}
-lemma sim_run_append [simp]:
-  assumes "(us,vs) \<in> sim_run r" and "(xs,ys) \<in> sim_run r"
-  shows "(us @ xs, vs @ ys) \<in> sim_run r"
-  using assms unfolding sim_run_def by (auto intro: list_all2_appendI)
+
+lemma div_sim_run_append [simp]:
+  assumes "(us,vs) \<in> div_sim_run r d" and "(xs,ys) \<in> div_sim_run r d"
+  shows "(us @ xs, vs @ ys) \<in> div_sim_run r d"
+  using assms unfolding div_sim_run_def by (auto intro: list_all2_appendI)
 
 text {*
   As a special case, appending two similar transitions to two similar runs
   yields again two similar runs.
 *}
-lemma sim_run_append_trans:
-  assumes "(ts, ts') \<in> sim_run r" and "(t, t') \<in> sim_transition r"
-  shows "(ts @ [t], ts' @ [t']) \<in> sim_run r"
+lemma div_sim_run_append_trans:
+  assumes "(ts, ts') \<in> div_sim_run r d" and "(t, t') \<in> div_sim_transition r d"
+  shows "(ts @ [t], ts' @ [t']) \<in> div_sim_run r d"
   using assms by simp
 
 text {*
@@ -241,49 +287,59 @@ text {*
   simulations between runs.
 *}
 
-theorem sim_run:
+theorem div_sim_run:
   assumes 
-    sim: "(l,l') \<in> simulation r" 
+    sim: "(l, l') \<in> div_simulation r" 
   and 
     ts: "ts \<in> runs l"
-  and
-    safe: "\<forall> t . t \<in> set ts \<and> t \<notin> div_trans l'"
-  obtains ts' where "ts' \<in> runs l'" "(ts,ts') \<in> sim_run r"
-proof -
-  from ts have "\<exists>ts' \<in> runs l'. (ts, ts') \<in> sim_run r"
+  obtains ts' where "ts' \<in> runs l'" "(ts,ts') \<in> div_sim_run r (divergences l')"
+sorry
+(*
+proof
+  from ts have "\<exists>ts' \<in> runs l'. (ts, ts') \<in> div_sim_run r (divergences l')"
   proof (induct)
-    show "\<exists>ts' \<in> runs l'. ([], ts') \<in> sim_run r" by (auto intro: runs.base)
+    show "\<exists>ts' \<in> runs l'. ([], ts') \<in> div_sim_run r (divergences l')" by (auto intro: runs.base)
   next
     fix t
     assume "t \<notin> div_trans l" "src t \<in> init l"
     with sim obtain t' where
-      "(src t, src t') \<in> r" "src t' \<in> init l'"
-      "t' \<notin> div_trans l'" "(t,t') \<in> sim_transition r"
-      unfolding simulation_def sorry
-    thus "\<exists>ts'\<in>runs l'. ([t], ts') \<in> sim_run r"
+      "src t' \<in> init l'"
+      "(src t, src t') \<in> r"
+      "src t' = src t"
+      "lbl t' = lbl t" 
+      "(t, t') \<in> div_sim_transition r (divergences l')"
+      unfolding div_simulation_def div_trans_def sorry
+    thus "\<exists>ts'\<in>runs l'. ([t], ts') \<in> div_sim_run r (divergences l')"
       by (auto intro: runs.start)
   next
     fix t ts
     assume t: "t \<notin> div_trans l" "src t = dst (last ts)"
        and ts: "ts \<in> runs l" "ts \<noteq> []"
-       and ih: "\<exists>ts'\<in>runs l'. (ts, ts') \<in> sim_run r"
-    from ih obtain ts' where ts': "ts' \<in> runs l'" "(ts,ts') \<in> sim_run r" by blast
+       and ih: "\<exists>ts'\<in>runs l'. (ts, ts') \<in> div_sim_run r (divergences l')"
+    from ih obtain ts' where ts': "ts' \<in> runs l'" "(ts,ts') \<in> div_sim_run r (divergences l')" by blast
     from ts ts' have "(dst (last ts), dst (last ts')) \<in> r"
-      by (metis sim_run_last_state)
+      by (metis div_sim_run_last_state)
     with sim t obtain t' where
-      t': "t' \<notin> div_trans l'" "src t' = dst (last ts')" "(t,t') \<in> sim_transition r"
-      unfolding simulation_def sorry
-    from ts ts' have "ts' \<noteq> []" by (simp add: sim_run_empty_iff)
+      t': "t' \<notin> div_trans l'" "src t' = dst (last ts')" "(t,t') \<in> div_sim_transition r (divergences l')"
+      unfolding div_simulation_def sorry
+    from ts ts' have "ts' \<noteq> []" by (simp add: div_sim_run_empty_iff)
     with ts' t' have "ts' @ [t'] \<in> runs l'" by (blast intro: runs.step)
-    with ts' t' show "\<exists>ts'\<in>runs l'. (ts @ [t], ts') \<in> sim_run r"
+    with ts' t' show "\<exists>ts'\<in>runs l'. (ts @ [t], ts') \<in> div_sim_run r (divergences l')"
       sorry
   qed
   with that show ?thesis by blast
 qed
+*)
 
-lemma sim_traces:
-  assumes sim: "(l,l') \<in> simulation r" and tev: "(t, ev) \<in> trace_div l"
-  shows "\<exists> (t', ev') \<in> trace_div l'. t = t' \<and> ev' \<subseteq> ev"
+lemma div_sim_traces_1:
+  assumes sim: "l \<preceq>\<preceq> l'" and tev: "(t, ev) \<in> trace_div l"
+  shows "\<exists> (t', ev') \<in> trace_div l'. t' = t \<or> 
+             (\<exists> e' \<in> ev' . (\<exists> t'' . t' @ [e'] @ t'' = t))"
+sorry
+
+lemma div_sim_traces_2:
+  assumes sim: "l \<preceq>\<preceq> l'" and tev: "(t', ev') \<in> trace_div l'"
+  shows "\<exists> (t, ev) \<in> trace_div l. t = t' \<and> ev \<supseteq> ev'"
 sorry
 
 (*
